cedar-lean/Cedar/Thm/SymCC/Opt.lean
@@ -158,17 +158,18 @@ theorem compile_ok_then_exists_wtps {ps : Policies} {cps : CompiledPolicies} {Γ
 
 /--
 This theorem covers the "happy path" -- showing that if optimized policy
-compilation succeeds, then `satAsserts?` and `satAssertsOpt?'` are equivalent.
+compilation with `CompiledPolicy.compile` succeeds, then `satAsserts?` and
+`satAssertsOpt?` are equivalent.
 -/
-theorem satAssertsOpt?'_eqv_satAsserts?_ok {ps wps : Policies} {cps : List CompiledPolicy} {Γ : Validation.TypeEnv} :
+theorem cp_satAssertsOpt?_eqv_satAsserts?_ok {ps wps : Policies} {cps : List CompiledPolicy} {Γ : Validation.TypeEnv} :
   ps.length = cps.length →
   cps ≠ [] →
   ps.mapM (CompiledPolicy.compile · Γ) = .ok cps →
   ps.mapM (wellTypedPolicy · Γ) = .ok wps →
-  satAsserts? wps asserts (SymEnv.ofTypeEnv Γ) = satAssertsOpt?' cps asserts
+  satAsserts? wps asserts (SymEnv.ofTypeEnv Γ) = satAssertsOpt? (cps.map CompiledPolicyₛ.policy) asserts
 := by
   intro hlen
-  simp [satAsserts?, satAssertsOpt?']
+  simp [satAsserts?, satAssertsOpt?]
   intro hnil hcps hwps
   have hεnv : ∀ cp ∈ cps, cp.εnv = SymEnv.ofTypeEnv Γ := by
     intro cp hcp
@@ -188,47 +189,58 @@ theorem satAssertsOpt?'_eqv_satAsserts?_ok {ps wps : Policies} {cps : List Compi
   simp [Functor.map, Except.map] at hcps
   split at hcps <;> simp at hcps
   replace ⟨hcps, htemp⟩ := hcps ; subst cp' htemp ; rename_i cps hcps ; have hcp := hcp' ; clear hcp'
+  simp only [CompiledPolicyₛ.εnv]
   rw [cp_compile_produces_the_right_env hcp]
   congr
   funext I
   cases I <;> simp only
   case some I =>
-  suffices SymEnv.extract? ((wp :: wps).map Policy.toExpr) I (SymEnv.ofTypeEnv Γ) = CompiledPolicy.extractOpt? (cp :: cps) I by rw [this] ; rfl
-  rw [cp_extractOpt?_eqv_extract? (εnv := cp.εnv) (by simp)]
+  suffices SymEnv.extract? ((wp :: wps).map Policy.toExpr) I (SymEnv.ofTypeEnv Γ) = extractOpt? (.policy cp :: cps.map CompiledPolicyₛ.policy) I by rw [this] ; rfl
+  rw [extractOpt?_eqv_extract? (εnv := cp.εnv) (by simp)]
   · congr 1
-    · simp only [List.map_cons, Function.comp_apply, List.cons.injEq]
+    · simp only [List.map_cons, List.flatMap_cons, CompiledPolicyₛ.allPolicies,
+        List.cons_append, List.nil_append, List.cons.injEq]
+      simp only [flatMap_allPolicies_policy, List.map_map]
       simp only [compiled_policy_eq_wtp hcp hwp, true_and]
       rw [← List.forall₂_iff_map_eq]
-      apply List.Forall₂.imp (R := λ a b => a = CompiledPolicy.policy b)
-      · intro a b h ; subst h ; simp
+      apply List.Forall₂.imp (R := λ a b => a = b.policy)
+      · intro a b h ; subst a ; simp
       · rw [List.mapM_ok_iff_forall₂] at hcps hwps
         apply List.forall₂_trans_ish hwps hcps
         intro p wp cp hwp hcp
         exact (compiled_policy_eq_wtp hcp hwp).symm
     · simp [cp_compile_produces_the_right_env hcp]
-  · intro cp' hcp'
-    cases hcp'
+  · intro cpₛ hcpₛ
+    cases hcpₛ
     · rfl
-    · rename_i hcp'
+    · rename_i hcpₛ
+      change cpₛ ∈ cps.map CompiledPolicyₛ.policy at hcpₛ
+      simp only [List.mem_map] at hcpₛ
+      replace ⟨cp', hcp', hcpₛ⟩ := hcpₛ ; subst cpₛ
       replace ⟨hεnv, hεnv'⟩ := hεnv
-      simp [hεnv, hεnv' cp' hcp']
-  · intro cp' hcp'
-    cases hcp'
+      simp [CompiledPolicyₛ.εnv, hεnv, hεnv' cp' hcp']
+  · intro cpₛ hcpₛ
+    cases hcpₛ
     · exists p, Γ
-    · rename_i hcp'
+    · rename_i hcpₛ
+      change cpₛ ∈ cps.map CompiledPolicyₛ.policy at hcpₛ
+      simp only [List.mem_map] at hcpₛ
+      replace ⟨cp', hcp', hcpₛ⟩ := hcpₛ ; subst cpₛ
+      simp only
       replace ⟨p', hp', hcps⟩ := List.mapM_ok_implies_all_from_ok hcps cp' hcp'
       exists p', Γ
 
 /--
 This theorem covers the "happy path" -- showing that if optimized policy
-compilation succeeds, then `satAsserts?` and `satAssertsOpt?` are equivalent.
+compilation with `CompiledPolicies.compile` succeeds, then `satAsserts?` and
+`satAssertsOpt?` are equivalent.
 -/
-theorem satAssertsOpt?_eqv_satAsserts?_ok {pss wpss : List Policies} {cpss : List CompiledPolicies} {Γ : Validation.TypeEnv} :
+theorem cps_satAssertsOpt?_eqv_satAsserts?_ok {pss wpss : List Policies} {cpss : List CompiledPolicies} {Γ : Validation.TypeEnv} :
   pss.length = cpss.length →
   cpss ≠ [] →
   pss.mapM (CompiledPolicies.compile · Γ) = .ok cpss →
   pss.mapM (wellTypedPolicies · Γ) = .ok wpss →
-  satAsserts? wpss.flatten asserts (SymEnv.ofTypeEnv Γ) = satAssertsOpt? cpss asserts
+  satAsserts? wpss.flatten asserts (SymEnv.ofTypeEnv Γ) = satAssertsOpt? (cpss.map CompiledPolicyₛ.policies) asserts
 := by
   intro hlen
   simp [satAsserts?, satAssertsOpt?]
@@ -251,15 +263,18 @@ theorem satAssertsOpt?_eqv_satAsserts?_ok {pss wpss : List Policies} {cpss : Lis
   simp [Functor.map, Except.map] at hcpss
   split at hcpss <;> simp at hcpss
   replace ⟨hcpss, htemp⟩ := hcpss ; subst cps' htemp ; rename_i cpss hcpss ; have hcps := hcps' ; clear hcps'
+  simp only [CompiledPolicyₛ.εnv]
   rw [cps_compile_produces_the_right_env hcps]
   congr
   funext I
   cases I <;> simp only
   case some I =>
-  suffices SymEnv.extract? (List.map (List.map Policy.toExpr) (wps :: wpss)).flatten I (SymEnv.ofTypeEnv Γ) = CompiledPolicies.extractOpt? (cps :: cpss) I by rw [this] ; rfl
-  rw [cps_extractOpt?_eqv_extract? (εnv := cps.εnv) (by simp)]
+  suffices SymEnv.extract? (List.map (List.map Policy.toExpr) (wps :: wpss)).flatten I (SymEnv.ofTypeEnv Γ) = extractOpt? (.policies cps :: cpss.map CompiledPolicyₛ.policies) I by rw [this] ; rfl
+  rw [extractOpt?_eqv_extract? (εnv := cps.εnv) (by simp)]
   · congr 1
-    · simp only [List.map_cons, List.flatten_cons, List.flatMap_cons, List.map_append]
+    · simp only [List.map_cons, List.flatten_cons, List.flatMap_cons, CompiledPolicyₛ.allPolicies,
+        List.map_append]
+      simp only [flatMap_allPolicies_policies]
       congr 2
       · simp [compiled_policies_eq_wtps hcps hwps]
       · simp [List.flatMap]
@@ -272,16 +287,22 @@ theorem satAssertsOpt?_eqv_satAsserts?_ok {pss wpss : List Policies} {cpss : Lis
           intro ps wps cps hwps hcps
           exact (compiled_policies_eq_wtps hcps hwps).symm
     · simp [cps_compile_produces_the_right_env hcps]
-  · intro cps' hcps'
-    cases hcps'
+  · intro cpₛ hcpₛ
+    cases hcpₛ
     · rfl
-    · rename_i hcps'
+    · rename_i hcpₛ
+      change cpₛ ∈ cpss.map CompiledPolicyₛ.policies at hcpₛ
+      simp only [List.mem_map] at hcpₛ
+      replace ⟨cps', hcps', hcpₛ⟩ := hcpₛ ; subst cpₛ
       replace ⟨hεnv, hεnv'⟩ := hεnv
-      simp [hεnv, hεnv' cps' hcps']
-  · intro cps' hcps'
-    cases hcps'
+      simp [CompiledPolicyₛ.εnv, hεnv, hεnv' cps' hcps']
+  · intro cpₛ hcpₛ
+    cases hcpₛ
     · exists ps, Γ
-    · rename_i hcps'
+    · rename_i hcpₛ
+      change cpₛ ∈ cpss.map CompiledPolicyₛ.policies at hcpₛ
+      simp only [List.mem_map] at hcpₛ
+      replace ⟨cps', hcps', hcpₛ⟩ := hcpₛ ; subst cpₛ
       replace ⟨ps', hps', hcpss⟩ := List.mapM_ok_implies_all_from_ok hcpss cps' hcps'
       exists ps', Γ
 
@@ -304,12 +325,12 @@ theorem neverErrorsOpt?_eqv_neverErrors?_ok {p : Policy} {cp : CompiledPolicy} {
   exists wp ; apply And.intro h₁
   have ⟨asserts, h₂⟩ := verifyNeverErrors_is_ok hwf h₁
   simp [h₂]
-  rw [← satAssertsOpt?'_eqv_satAsserts?_ok (ps := [p]) (cps := [cp]) (by simp) (by simp)]
+  rw [cp_satAssertsOpt?_eqv_satAsserts?_ok (ps := [p]) (cps := [cp]) (by simp) (by simp)]
   · have := verifyNeverErrorsOpt_eqv_verifyNeverErrors_ok h₀ h₁
     simp [h₂, ResultAssertsEquiv] at this
-    exact Asserts.Equiv.satAsserts? [wp] _ (Asserts.Equiv.symm this)
-  · simp [pure, Except.pure, h₀]
-  · simp [pure, Except.pure, h₁]
+    exact Asserts.Equiv.satAssertsOpt? [.policy cp] (Asserts.Equiv.symm this)
+  · simp [h₀]
+  · simp [h₁]
 
 /--
 This theorem covers the "happy path" -- showing that if optimized policy
@@ -330,12 +351,12 @@ theorem alwaysMatchesOpt?_eqv_alwaysMatches?_ok {p : Policy} {cp : CompiledPolic
   exists wp ; apply And.intro h₁
   have ⟨asserts, h₂⟩ := verifyAlwaysMatches_is_ok hwf h₁
   simp [h₂]
-  rw [← satAssertsOpt?'_eqv_satAsserts?_ok (ps := [p]) (cps := [cp]) (by simp) (by simp)]
+  rw [cp_satAssertsOpt?_eqv_satAsserts?_ok (ps := [p]) (cps := [cp]) (by simp) (by simp)]
   · have := verifyAlwaysMatchesOpt_eqv_verifyAlwaysMatches_ok h₀ h₁
     simp [h₂, ResultAssertsEquiv] at this
-    exact Asserts.Equiv.satAsserts? [wp] _ (Asserts.Equiv.symm this)
-  · simp [pure, Except.pure, h₀]
-  · simp [pure, Except.pure, h₁]
+    exact Asserts.Equiv.satAssertsOpt? [.policy cp] (Asserts.Equiv.symm this)
+  · simp [h₀]
+  · simp [h₁]
 
 /--
 This theorem covers the "happy path" -- showing that if optimized policy
@@ -356,12 +377,12 @@ theorem neverMatchesOpt?_eqv_neverMatches?_ok {p : Policy} {cp : CompiledPolicy}
   exists wp ; apply And.intro h₁
   have ⟨asserts, h₂⟩ := verifyNeverMatches_is_ok hwf h₁
   simp [h₂]
-  rw [← satAssertsOpt?'_eqv_satAsserts?_ok (ps := [p]) (cps := [cp]) (by simp) (by simp)]
+  rw [cp_satAssertsOpt?_eqv_satAsserts?_ok (ps := [p]) (cps := [cp]) (by simp) (by simp)]
   · have := verifyNeverMatchesOpt_eqv_verifyNeverMatches_ok h₀ h₁
     simp [h₂, ResultAssertsEquiv] at this
-    exact Asserts.Equiv.satAsserts? [wp] _ (Asserts.Equiv.symm this)
-  · simp [pure, Except.pure, h₀]
-  · simp [pure, Except.pure, h₁]
+    exact Asserts.Equiv.satAssertsOpt? [.policy cp] (Asserts.Equiv.symm this)
+  · simp [h₀]
+  · simp [h₁]
 
 /--
 This theorem covers the "happy path" -- showing that if optimized policy
@@ -381,12 +402,12 @@ theorem matchesEquivalentOpt?_eqv_matchesEquivalent?_ok {p₁ p₂ wp₁ wp₂ :
   intro hwf h₀ h₁ h₂ h₃
   have ⟨asserts, h₄⟩ := verifyMatchesEquivalent_is_ok hwf h₂ h₃
   simp only [h₄]
-  rw [← satAssertsOpt?'_eqv_satAsserts?_ok (ps := [p₁, p₂]) (cps := [cp₁, cp₂]) (by simp) (by simp)]
+  rw [cp_satAssertsOpt?_eqv_satAsserts?_ok (ps := [p₁, p₂]) (cps := [cp₁, cp₂]) (by simp) (by simp)]
   · have := verifyMatchesEquivalentOpt_eqv_verifyMatchesEquivalent_ok h₀ h₁ h₂ h₃
     simp [h₄, ResultAssertsEquiv] at this
-    exact Asserts.Equiv.satAsserts? [wp₁, wp₂] _ (Asserts.Equiv.symm this)
-  · simp [pure, Except.pure, h₀, h₁]
-  · simp [pure, Except.pure, h₂, h₃]
+    exact Asserts.Equiv.satAssertsOpt? [.policy cp₁, .policy cp₂] (Asserts.Equiv.symm this)
+  · simp [h₀, h₁]
+  · simp [h₂, h₃]
 
 /--
 This theorem covers the "happy path" -- showing that if optimized policy
@@ -406,12 +427,12 @@ theorem matchesImpliesOpt?_eqv_matchesImplies?_ok {p₁ p₂ wp₁ wp₂ : Polic
   intro hwf h₀ h₁ h₂ h₃
   have ⟨asserts, h₄⟩ := verifyMatchesImplies_is_ok hwf h₂ h₃
   simp only [h₄]
-  rw [← satAssertsOpt?'_eqv_satAsserts?_ok (ps := [p₁, p₂]) (cps := [cp₁, cp₂]) (by simp) (by simp)]
+  rw [cp_satAssertsOpt?_eqv_satAsserts?_ok (ps := [p₁, p₂]) (cps := [cp₁, cp₂]) (by simp) (by simp)]
   · have := verifyMatchesImpliesOpt_eqv_verifyMatchesImplies_ok h₀ h₁ h₂ h₃
     simp [h₄, ResultAssertsEquiv] at this
-    exact Asserts.Equiv.satAsserts? [wp₁, wp₂] _ (Asserts.Equiv.symm this)
-  · simp [pure, Except.pure, h₀, h₁]
-  · simp [pure, Except.pure, h₂, h₃]
+    exact Asserts.Equiv.satAssertsOpt? [.policy cp₁, .policy cp₂] (Asserts.Equiv.symm this)
+  · simp [h₀, h₁]
+  · simp [h₂, h₃]
 
 /--
 This theorem covers the "happy path" -- showing that if optimized policy
@@ -431,12 +452,12 @@ theorem matchesDisjointOpt?_eqv_matchesDisjoint?_ok {p₁ p₂ wp₁ wp₂ : Pol
   intro hwf h₀ h₁ h₂ h₃
   have ⟨asserts, h₄⟩ := verifyMatchesDisjoint_is_ok hwf h₂ h₃
   simp only [h₄]
-  rw [← satAssertsOpt?'_eqv_satAsserts?_ok (ps := [p₁, p₂]) (cps := [cp₁, cp₂]) (by simp) (by simp)]
+  rw [cp_satAssertsOpt?_eqv_satAsserts?_ok (ps := [p₁, p₂]) (cps := [cp₁, cp₂]) (by simp) (by simp)]
   · have := verifyMatchesDisjointOpt_eqv_verifyMatchesDisjoint_ok h₀ h₁ h₂ h₃
     simp [h₄, ResultAssertsEquiv] at this
-    exact Asserts.Equiv.satAsserts? [wp₁, wp₂] _ (Asserts.Equiv.symm this)
-  · simp [pure, Except.pure, h₀, h₁]
-  · simp [pure, Except.pure, h₂, h₃]
+    exact Asserts.Equiv.satAssertsOpt? [.policy cp₁, .policy cp₂] (Asserts.Equiv.symm this)
+  · simp [h₀, h₁]
+  · simp [h₂, h₃]
 
 /--
 Full equivalence for `neverErrors?` and `neverErrorsOpt?`, including both the
@@ -662,13 +683,14 @@ theorem impliesOpt?_eqv_implies?_ok {ps₁ ps₂ : Policies} {cps₁ cps₂ : Co
   exists wps₂ ; apply And.intro hwps₂
   have ⟨asserts, h₁⟩ := verifyImplies_is_ok hwf hwps₁ hwps₂
   simp [h₁]
-  rw [← satAssertsOpt?_eqv_satAsserts?_ok (pss := [ps₁, ps₂]) (wpss := [wps₁, wps₂]) (cpss := [cps₁, cps₂]) (by simp) (by simp)]
+  have := cps_satAssertsOpt?_eqv_satAsserts?_ok (pss := [ps₁, ps₂]) (wpss := [wps₁, wps₂]) (cpss := [cps₁, cps₂]) (asserts := asserts) (Γ := Γ) (by simp) (by simp)
+  simp only [List.flatten_cons, List.flatten_nil, List.append_nil, List.map_cons, List.map_nil] at this
+  rw [this] ; clear this
   · have := verifyImpliesOpt_eqv_verifyImplies_ok hcps₁ hcps₂ hwps₁ hwps₂
     simp [h₁, ResultAssertsEquiv] at this
-    simp only [List.flatten, List.append_eq, List.append_nil]
-    exact Asserts.Equiv.satAsserts? (wps₁ ++ wps₂) _ (Asserts.Equiv.symm this)
-  · simp [pure, Except.pure, hcps₁, hcps₂]
-  · simp [pure, Except.pure, hwps₁, hwps₂]
+    exact Asserts.Equiv.satAssertsOpt? [.policies cps₁, .policies cps₂] (Asserts.Equiv.symm this)
+  · simp [hcps₁, hcps₂]
+  · simp [hwps₁, hwps₂]
 
 /--
 Full equivalence for `implies?` and `impliesOpt?`, including both the
@@ -726,13 +748,14 @@ theorem alwaysAllowsOpt?_eqv_alwaysAllows?_ok {ps : Policies} {cps : CompiledPol
   exists wps ; apply And.intro hwps
   have ⟨asserts, h₁⟩ := verifyAlwaysAllows_is_ok hwf hwps
   simp [h₁]
-  rw [← satAssertsOpt?_eqv_satAsserts?_ok (pss := [ps]) (wpss := [wps]) (cpss := [cps]) (Γ := Γ) (by simp) (by simp)]
+  have := cps_satAssertsOpt?_eqv_satAsserts?_ok (pss := [ps]) (wpss := [wps]) (cpss := [cps]) (asserts := asserts) (Γ := Γ) (by simp) (by simp)
+  simp only [List.flatten_cons, List.flatten_nil, List.append_nil, List.map_cons, List.map_nil] at this
+  rw [this] ; clear this
   · have := verifyAlwaysAllowsOpt_eqv_verifyAlwaysAllows_ok hcps hwps
     simp [h₁, ResultAssertsEquiv] at this
-    simp only [List.flatten, List.append_eq, List.append_nil]
-    exact Asserts.Equiv.satAsserts? wps _ (Asserts.Equiv.symm this)
-  · simp [pure, Except.pure, hcps]
-  · simp [pure, Except.pure, hwps]
+    exact Asserts.Equiv.satAssertsOpt? [.policies cps] (Asserts.Equiv.symm this)
+  · simp [hcps]
+  · simp [hwps]
 
 /--
 Full equivalence for `alwaysAllows?` and `alwaysAllowsOpt?`, including both the
@@ -782,13 +805,14 @@ theorem alwaysDeniesOpt?_eqv_alwaysDenies?_ok {ps : Policies} {cps : CompiledPol
   exists wps ; apply And.intro hwps
   have ⟨asserts, h₁⟩ := verifyAlwaysDenies_is_ok hwf hwps
   simp [h₁]
-  rw [← satAssertsOpt?_eqv_satAsserts?_ok (pss := [ps]) (wpss := [wps]) (cpss := [cps]) (Γ := Γ) (by simp) (by simp)]
+  have := cps_satAssertsOpt?_eqv_satAsserts?_ok (pss := [ps]) (wpss := [wps]) (cpss := [cps]) (asserts := asserts) (Γ := Γ) (by simp) (by simp)
+  simp only [List.flatten_cons, List.flatten_nil, List.append_nil, List.map_cons, List.map_nil] at this
+  rw [this] ; clear this
   · have := verifyAlwaysDeniesOpt_eqv_verifyAlwaysDenies_ok hcps hwps
     simp [h₁, ResultAssertsEquiv] at this
-    simp only [List.flatten, List.append_eq, List.append_nil]
-    exact Asserts.Equiv.satAsserts? wps _ (Asserts.Equiv.symm this)
-  · simp [pure, Except.pure, hcps]
-  · simp [pure, Except.pure, hwps]
+    exact Asserts.Equiv.satAssertsOpt? [.policies cps] (Asserts.Equiv.symm this)
+  · simp [hcps]
+  · simp [hwps]
 
 /--
 Full equivalence for `alwaysDenies?` and `alwaysDeniesOpt?`, including both the
@@ -842,13 +866,14 @@ theorem equivalentOpt?_eqv_equivalent?_ok {ps₁ ps₂ : Policies} {cps₁ cps�
   exists wps₂ ; apply And.intro hwps₂
   have ⟨asserts, h₁⟩ := verifyEquivalent_is_ok hwf hwps₁ hwps₂
   simp [h₁]
-  rw [← satAssertsOpt?_eqv_satAsserts?_ok (pss := [ps₁, ps₂]) (wpss := [wps₁, wps₂]) (cpss := [cps₁, cps₂]) (by simp) (by simp)]
+  have := cps_satAssertsOpt?_eqv_satAsserts?_ok (pss := [ps₁, ps₂]) (wpss := [wps₁, wps₂]) (cpss := [cps₁, cps₂]) (asserts := asserts) (Γ := Γ) (by simp) (by simp)
+  simp only [List.flatten_cons, List.flatten_nil, List.append_nil, List.map_cons, List.map_nil] at this
+  rw [this] ; clear this
   · have := verifyEquivalentOpt_eqv_verifyEquivalent_ok hcps₁ hcps₂ hwps₁ hwps₂
     simp [h₁, ResultAssertsEquiv] at this
-    simp only [List.flatten, List.append_eq, List.append_nil]
-    exact Asserts.Equiv.satAsserts? (wps₁ ++ wps₂) _ (Asserts.Equiv.symm this)
-  · simp [pure, Except.pure, hcps₁, hcps₂]
-  · simp [pure, Except.pure, hwps₁, hwps₂]
+    exact Asserts.Equiv.satAssertsOpt? [.policies cps₁, .policies cps₂] (Asserts.Equiv.symm this)
+  · simp [hcps₁, hcps₂]
+  · simp [hwps₁, hwps₂]
 
 /--
 Full equivalence for `equivalent?` and `equivalentOpt?`, including both the
@@ -910,13 +935,14 @@ theorem disjointOpt?_eqv_disjoint?_ok {ps₁ ps₂ : Policies} {cps₁ cps₂ : 
   exists wps₂ ; apply And.intro hwps₂
   have ⟨asserts, h₁⟩ := verifyDisjoint_is_ok hwf hwps₁ hwps₂
   simp [h₁]
-  rw [← satAssertsOpt?_eqv_satAsserts?_ok (pss := [ps₁, ps₂]) (wpss := [wps₁, wps₂]) (cpss := [cps₁, cps₂]) (by simp) (by simp)]
+  have := cps_satAssertsOpt?_eqv_satAsserts?_ok (pss := [ps₁, ps₂]) (wpss := [wps₁, wps₂]) (cpss := [cps₁, cps₂]) (asserts := asserts) (Γ := Γ) (by simp) (by simp)
+  simp only [List.flatten_cons, List.flatten_nil, List.append_nil, List.map_cons, List.map_nil] at this
+  rw [this] ; clear this
   · have := verifyDisjointOpt_eqv_verifyDisjoint_ok hcps₁ hcps₂ hwps₁ hwps₂
     simp [h₁, ResultAssertsEquiv] at this
-    simp only [List.flatten, List.append_eq, List.append_nil]
-    exact Asserts.Equiv.satAsserts? (wps₁ ++ wps₂) _ (Asserts.Equiv.symm this)
-  · simp [pure, Except.pure, hcps₁, hcps₂]
-  · simp [pure, Except.pure, hwps₁, hwps₂]
+    exact Asserts.Equiv.satAssertsOpt? [.policies cps₁, .policies cps₂] (Asserts.Equiv.symm this)
+  · simp [hcps₁, hcps₂]
+  · simp [hwps₁, hwps₂]
 
 /--
 Full equivalence for `disjoint?` and `disjointOpt?`, including both the
